Added proof for bracketed-usage.

checker/cumulative.v
@@ -3,6 +3,7 @@ Require Import Bool.
 Require Import bounds.
 Require Import prim.
 Require Import Program.
+Require Import Recdef.
 Require Import Program.Wf.
 
 Local Open Scope nat_scope.
@@ -31,16 +32,15 @@ Definition eval_start (t : task) (theta : asg) :=
 Definition eval_end (t : task) (theta : asg) :=
   Zplus (eval_ivar t.(svar) theta) (Z_of_nat t.(duration)).
 
-Definition task_at_time (t : task) (time : nat) (theta : asg) : nat :=
+Definition task_at_time (t : task) (time : Z) (theta : asg) : nat :=
   let tstart := eval_start t theta in
   let tend := eval_end t theta in
-  let ztime := Z_of_nat time in
-  if Z_leb tstart ztime && Z_ltb ztime tend then
+  if Z_leb tstart time && Z_ltb time tend then
     t.(resource)
   else
     0%nat.
 
-Fixpoint eval_usage (ts : list task) (time : nat) (theta : asg) : nat :=
+Fixpoint eval_usage (ts : list task) (time : Z) (theta : asg) : nat :=
   match ts with
   | nil => 0%nat
   | cons t ts' =>
@@ -48,17 +48,17 @@ Fixpoint eval_usage (ts : list task) (time : nat) (theta : asg) : nat :=
   end.
 
 Definition eval_cumul (c : cumul) (theta : asg) :=
-  forall (time : nat), le (eval_usage c.(tasks) time theta) c.(limit).
+  forall (time : Z), le (eval_usage c.(tasks) time theta) c.(limit).
 
-Fixpoint span_usage (ts : list task) (start : nat) (sz : nat) (theta : asg) :=
+Fixpoint span_usage (ts : list task) (start : Z) (sz : nat) (theta : asg) :=
   match sz with
   | O => 0%nat
   | S sz' =>
-     plus (eval_usage ts (start+sz-1) theta) (span_usage ts start sz' theta)
+     plus (eval_usage ts (start+(Z_of_nat sz)-1) theta) (span_usage ts start sz' theta)
   end.
 
 Theorem  span_usage_lim :
-  forall (c : cumul) (start : nat) (sz : nat) (theta : asg),
+  forall (c : cumul) (start : Z) (sz : nat) (theta : asg),
     eval_cumul c theta ->
       le (span_usage c.(tasks) start sz theta) (c.(limit) * sz).
 Proof.
@@ -67,7 +67,7 @@ Proof.
     unfold span_usage. omega.
 
     unfold span_usage; fold span_usage.
-    assert (le (eval_usage (tasks c) (start + (S sz) - 1) theta) c.(limit)).
+    assert (le (eval_usage (tasks c) (start + (Z_of_nat (S sz)) - 1) theta) c.(limit)).
     apply H.
     rewrite <- mult_n_Sm.
     rewrite plus_comm.
@@ -76,7 +76,7 @@ Proof.
     exact H0.
 Qed.
 
-Theorem span_usage_split : forall (t : task) (ts : list task) (start sz : nat) (theta : asg),
+Theorem span_usage_split : forall (t : task) (ts : list task) (start : Z) (sz : nat) (theta : asg),
   span_usage (cons t ts) start sz theta =
     plus (span_usage (cons t nil) start sz theta) (span_usage ts start sz theta).
 Proof.
@@ -90,14 +90,14 @@ Proof.
     unfold eval_usage at 1; fold eval_usage. unfold eval_usage at 2.
     rewrite IHsz. omega.
 Qed.
-    
-Fixpoint task_usage (t : task) (start : nat) (sz : nat) (theta : asg) :=
+ 
+Fixpoint task_usage (t : task) (start : Z) (sz : nat) (theta : asg) :=
   match sz with
   | O => 0%nat
   | S sz' =>
-    plus (task_at_time t (start+sz-1) theta) (task_usage t start sz' theta)
+    plus (task_at_time t (start+(Z_of_nat sz)-1) theta) (task_usage t start sz' theta)
   end.
-Theorem task_usage_eq_span : forall (t : task) (start sz : nat) (theta : asg),
+Theorem task_usage_eq_span : forall (t : task) (start : Z) (sz : nat) (theta : asg),
   task_usage t start sz theta = span_usage (cons t nil) start sz theta.
 Proof.
   intros; induction sz.
@@ -106,38 +106,141 @@ Proof.
     unfold task_usage, span_usage. fold task_usage; fold span_usage.
     rewrite <- IHsz. unfold eval_usage. omega.
 Qed.
-Theorem task_in_span : forall (t : task) (time : nat) (theta : asg),
-  Zle (eval_start t theta) (Z_of_nat time)
-    /\ Zlt (Z_of_nat time) (eval_end t theta) ->
+Definition in_span (t : task) (time : Z) (theta : asg) :=
+  Zle (eval_start t theta) time /\ Zlt time (eval_end t theta).
+
+Theorem task_in_span : forall (t : task) (time : Z) (theta : asg),
+  in_span t time theta ->
       task_at_time t time theta = t.(resource).
 Proof.
   intros; destruct H as [Hs He].
-  unfold task_at_time.
-  assert (Z_leb (eval_start t theta) (Z_of_nat time)
-    && Z_ltb (Z_of_nat time) (eval_end t theta) = true) as Ht.
+  unfold in_span, task_at_time.
+  assert (Z_leb (eval_start t theta) time
+    && Z_ltb time (eval_end t theta) = true) as Ht.
     apply andb_true_iff; rewrite Z_leb_iff_le; rewrite Z_ltb_iff_lt.
     omega.
   destruct andb.
     trivial.
     discriminate.
 Qed.
-Theorem task_usage_monotone_r : forall (t : task) (start sz sz' : nat) (theta : asg),
-  le sz sz' -> le (task_usage t start sz theta) (task_usage t start sz' theta).
+Theorem task_duration_usage : forall (t : task) (sz : nat) (theta : asg),
+  sz <= t.(duration) ->
+    task_usage t (eval_start t theta) sz theta = t.(resource)*sz.
+Proof.
+  intros; induction sz.
+    unfold task_usage; omega.
+
+    unfold task_usage; fold task_usage.
+    assert (in_span t (Zminus (Zplus (eval_start t theta) (Z_of_nat (S sz))) 1) theta).
+      unfold in_span, eval_start, eval_end.
+      assert (Zlt (Z_of_nat sz) (Z_of_nat t.(duration))).
+        omega.
+      rewrite inj_S;  omega.
+    rewrite task_in_span.
+    rewrite IHsz.
+    rewrite mult_succ_r; rewrite plus_comm; trivial.
+    omega.
+    exact H0.
+Qed.
+
+Theorem task_usage_split :
+  forall (t : task) (lb : Z) (sz sz' : nat) (theta : asg),
+  task_usage t lb sz theta +
+    task_usage t (Zplus lb (Z_of_nat sz)) sz' theta
+  = task_usage t lb (sz + sz') theta.
+Proof.
+  intros. induction sz'.
+  unfold task_usage at 2 3. fold task_usage.
+  repeat (rewrite <- plus_n_O); trivial.
+
+  rewrite <- plus_n_Sm.
+  unfold task_usage; fold task_usage.
+  repeat (rewrite inj_S). repeat (rewrite inj_plus).
+  repeat (rewrite <- Zplus_succ_r).
+  repeat (rewrite <- Zplus_assoc). omega.
+Qed.
+
+Definition task_usageZ (t : task) (lb ub : Z) (theta : asg) :=
+  if Z_le_dec lb ub then
+    task_usage t lb (Zabs_nat (Zminus ub lb)) theta
+  else
+    O.
+
+Theorem task_usageZ_eq :
+  forall (t : task) (lb : Z) (sz : nat) (theta : asg),
+    task_usage t lb sz theta = 
+    task_usageZ t lb (Zplus lb (Z_of_nat sz)) theta.
+Proof.
+  intros. unfold task_usageZ.
+  assert (Zle lb (lb + Z_of_nat sz)). omega.
+  destruct (Z_le_dec lb (Zplus lb (Z_of_nat sz))).
+  rewrite Zminus_plus.
+  rewrite Zabs_nat_Z_of_nat. trivial.
+  tauto.
+Qed.
+
+Theorem task_usageZ_split :
+  forall (t : task) (lb mid ub : Z) (theta : asg),
+    Zle lb mid /\ Zle mid ub ->
+    task_usageZ t lb mid theta + task_usageZ t mid ub theta
+      = task_usageZ t lb ub theta.
 Proof.
   intros.
-  induction sz'.
-    assert (sz = 0%nat) as Hsz0. omega.
-    rewrite Hsz0; trivial.
-    
-    assert (sz = (S sz') \/ sz < S sz'). omega.
-    destruct H0 as [Heq | Hlt].
-      rewrite Heq. omega.
-
-      unfold task_usage at 2;  fold task_usage.
-      assert (le O (task_at_time t (start + S sz' - 1) theta)). omega.
-      assert (forall (i j k : nat), i <= k -> i <= j + k). intros; omega. 
-      apply H1. apply IHsz'. apply lt_n_Sm_le. exact Hlt.
+    assert (mid = (Zplus lb (Z_of_nat (Zabs_nat (Zminus mid lb))))).
+    rewrite inj_Zabs_nat;
+    rewrite Zabs_eq. omega. omega.
+    assert (ub = (Zplus mid (Z_of_nat (Zabs_nat (Zminus ub mid))))).
+    rewrite inj_Zabs_nat; rewrite Zabs_eq. omega. omega.
+    assert (ub = (Zplus lb (Z_of_nat (Zabs_nat (Zminus ub lb))))).
+    rewrite inj_Zabs_nat; rewrite Zabs_eq. omega. omega.
+  rewrite H2 at 2; rewrite H1, H0.
+  repeat (rewrite <- task_usageZ_eq).
+  Check task_usage_split.
+  repeat (rewrite inj_Zabs_nat).
+  repeat (rewrite Zabs_eq).
+  repeat (rewrite Zplus_minus).
+  rewrite H0 at 2.
+  Check task_usage_split.
+  assert (Zabs_nat (ub - lb) = (Zabs_nat (mid - lb)) + (Zabs_nat (ub - mid))).
+  omega.
+  rewrite H3.
+  apply task_usage_split.
+  omega.
+  omega.
 Qed.
+  
+Definition task_bracketed (t : task) (lb ub : Z) (theta : asg) :=
+  Zle lb (eval_start t theta)
+    /\ Zlt (eval_end t theta) ub.
+
+Theorem task_bracketed_usageZ :
+  forall (t : task) (lb ub : Z) (theta : asg),
+    task_bracketed t lb ub theta ->
+      mult t.(resource) t.(duration) <= task_usageZ t lb ub theta.
+Proof.
+  unfold task_bracketed; intros.
+  destruct H as [Hs He].
+  unfold eval_end in He.
+  Check task_usageZ_split.
+  rewrite <- task_usageZ_split with (mid := (eval_start t theta)).
+  rewrite plus_comm.
+  apply le_plus_trans.
+  rewrite <- task_usageZ_split with (mid := (eval_end t theta)).
+  apply le_plus_trans.
+  unfold eval_end.
+  assert (eval_ivar (svar t) theta = eval_start t theta) as Hstart.
+    unfold eval_start; trivial.
+  rewrite Hstart.
+  rewrite <- task_usageZ_eq.
+  rewrite task_duration_usage.
+  omega.
+  omega.
+  unfold eval_start, eval_end.
+  omega.
+  unfold eval_start in *.
+  omega.
+Qed.
+  
 (*
 Theorem task_duration_usage : forall (t : task) (start sz : nat) (theta : asg),
   (Z_ge (Z_of_nat start) (eval_ivar t.(svar) theta) /\
